Use ExtLib for monads and monad transformers
Makes things much nicer, have real monad transformers
Do not get nice notations unless we want Obj.magic everywhere
Have to manually specify instances (need anyway for extraction)

src/util/StateMonad.v
@@ -1,11 +1,27 @@
 (*Several different state monads, which are extracted
   to mutable references in OCaml*)
 Require CoqBigInt.
+Require Import ErrorMonad.
 Require Import Monad.
-From stdpp Require Import base.
+Require Import Hashtbl. (*NOTE: stdpp and coq-ext-lib cannot both
+  be imported in same file!*)
+From ExtLib Require Import Monads MonadState StateMonad EitherMonad.
+Import MonadNotation.
+
+(*We use coq-ext-lib's monads and monad transformers.
+  (TODO) THis leads to bad OCaml code, but doing it ourselves
+    is very painful.
+  Because we extract to mutable references (with names), we make
+  each use of state a different set of definitions.
+  (TODO: can we improve this and reduce duplication>)*)
+
+(*From stdpp Require Import base.*)
+
+
+
 
 (*Generalized state monad*)
-Definition state (s a: Type) : Type := s -> (s * a).
+(*Definition state (s a: Type) : Type := s -> (s * a).
 Definition st_get {s: Type} : state s s := fun x => (x, x).
 Definition st_set {s: Type} (x: s) : state s unit := fun _ => (x, tt).
 Definition st_ret {s a: Type} (x: a) : state s a := fun s => (s, x).
@@ -33,9 +49,9 @@ Definition st_set2 {s1 s2: Type} (x: s2) : state_multi s1 s2 unit :=
   (fun y => ((fst y, x), tt)).
 Definition st_multi_ret {s1 s2 a: Type} (x: a) : state_multi s1 s2 a := st_ret x.
 Definition st_multi_bnd {s1 s2 a b: Type} (f: a -> state_multi s1 s2 b)
-  (m: state_multi s1 s2 a) : state_multi s1 s2 b := st_bnd f m.
+  (m: state_multi s1 s2 a) : state_multi s1 s2 b := st_bnd f m.*)
 
-(*Combine state and error handling (monad transformer)*)
+(*Combine state and error handling (monad transformer)
 Require Import ErrorMonad.
 
 (*We can't do monad transformers generically or else OCaml
@@ -57,78 +73,78 @@ Definition exceptT_bnd {s a b: Type} (f: a -> exceptT s b)
 Definition exceptT_lift {s a: Type} (x: state s a) : exceptT s a :=
   st_bnd (fun s => st_ret (ret s)) x.
 Definition exceptT_lift2 {s a: Type} (x: errorM a) : exceptT s a :=
-  st_ret x.
-
-(*And now we include several kinds of state:*)
-(* 1. A mutable counter*)
-(*Definition ctr (a: Type) : Type := state CoqBigInt.t a.
-Definition ctr_get : ctr CoqBigInt.t := st_get.
-Definition ctr_ret {a: Type} (x: a) : ctr a := st_ret x.
-Definition ctr_bnd {a b: Type} (f: a -> ctr b) (m: ctr a) : ctr b := st_bnd f m.
-(*2 hacks: to create a new counter (which starts at the given value)
-  and a vile hack to ensure that we can set the type of the creation*)
-Definition new_ctr (i: CoqBigInt.t) : ctr unit := st_set i.
-(*TODO: see if we need this*)
-Definition incr : ctr unit := ctr_bnd 
-  (fun i => st_set (CoqBigInt.succ i)) ctr_get.
-Definition ctr_unit := ctr unit.
-Definition ctr_list {A: Type} (l: list (ctr A)) : ctr (list A) :=
-  listM ctr_ret ctr_bnd l.*)
-Notation ctr a := (state CoqBigInt.t a).
-Notation ctr_bnd := st_bnd.
-Notation ctr_ret := st_ret.
-Notation ctr_get := st_get.
-Notation ctr_set := st_set.
+  st_ret x.*)
+Local Open Scope monad_scope.
+Existing Instance
+     Monad_state.
+(*Mutable counter*)
+Definition ctr a := (state CoqBigInt.t a).
+Global Instance Monad_ctr: Monad ctr := Monad_state _.
+Global Instance MonadState_ctr : MonadState CoqBigInt.t ctr := MonadState_state _.
+Definition ctr_bnd {a b} (f: a -> ctr b) (m: ctr a) : ctr b := 
+  bind m f.
+Definition ctr_ret {a} (x: a) : ctr a := ret x.
+Definition ctr_get : ctr CoqBigInt.t := get.
+Definition ctr_set (i: CoqBigInt.t) : ctr unit := put i.
 Definition ctr_ty := ctr unit.
-Definition new_ctr (i: CoqBigInt.t) : ctr unit := st_set i.
+Definition new_ctr (i: CoqBigInt.t) : ctr unit := put i.
 (*TODO: see if notation/inlined/whatever*)
 Definition ctr_incr : ctr unit :=
-  ctr_bnd (fun i => ctr_set (CoqBigInt.succ i)) ctr_get.
-
+  i <- ctr_get ;; ctr_set (CoqBigInt.succ i).
 (*2. Hash table*)
-Require Import Hashtbl.
+
+Existing Instance
+     Monad_stateT.
 Section HashTbl.
 Definition hash_st (key value a: Type) : Type := state (hashtbl key value) a.
-
+Global Instance Monad_hash_st key value: Monad (hash_st key value) := Monad_state _. 
+Global Instance MonadState_hash_st key value : 
+  MonadState (hashtbl key value) (hash_st key value) := MonadState_state _.
 Context {key value: Type} (hash: key -> CoqBigInt.t) 
   (eqb: key -> key -> bool).
 
-Definition hash_get (a: Type) : hash_st key value (hashtbl key value):= st_get.
+Definition hash_get (a: Type) : hash_st key value (hashtbl key value):= get.
 Definition hash_set (a: Type) (x: hashtbl key value) : hash_st key value unit :=
-  st_set x.
-Definition hash_ret {a: Type} (x: a) : hash_st key value a := st_ret x.
+  put x.
+Definition hash_ret {a: Type} (x: a) : hash_st key value a := ret x.
+(*TODO: change to notations or don't include at all?
+  No, Need definitions for extraction*)
 Definition hash_bnd {a b: Type} (f: a -> hash_st key value b) 
-  (m: hash_st key value a) : hash_st key value b :=
-  st_bnd f m.
-Definition new_hash : hash_st key value unit := st_set (create_hashtbl value).
+  (m: hash_st key value a) : hash_st key value b := bind m f.
+Definition new_hash : hash_st key value unit := put (create_hashtbl value).
 Definition hash_unit := hash_st key value unit.
 Definition hash_listM {A: Type} (l: list (hash_st key value A))
  := listM hash_ret hash_bnd l.
 End HashTbl.
 
 (*3. Hash consing - combine 2 states*)
-Notation hashcons_st key a :=
-  (state_multi CoqBigInt.t (hashset key) a).
+Definition hashcons_st key a := (state (CoqBigInt.t * hashset key) a).
+Global Instance Monad_hashcons_st key: Monad (hashcons_st key) := Monad_state _. 
+Global Instance MonadState_hashcons_st key : 
+  MonadState (CoqBigInt.t * hashset key) (hashcons_st key) := MonadState_state _.
 Definition hashcons_new key : hashcons_st key unit :=
-  fun _ => (CoqBigInt.one, create_hashset, tt).
-
-Notation hashcons_bnd := st_multi_bnd.
-Notation hashcons_ret := st_multi_ret.
+  put (CoqBigInt.one, create_hashset).
+Definition hashcons_bnd {key a b} (f: a -> hashcons_st key b) (m: hashcons_st key a) :
+  hashcons_st key b := bind m f.
+Definition hashcons_ret {key a} (x: a) : hashcons_st key a := ret x.
 (*TODO: if we do definitions, can we inline?*)
 Section HashCons.
 Context {key: Type} (hash: key -> CoqBigInt.t) 
   (eqb: key -> key -> bool).
 Definition hashcons_lookup (k: key) : hashcons_st key (option key) :=
-  hashcons_bnd (fun h => hashcons_ret (find_opt_hashset hash eqb h k)) 
-    st_get2.
-Definition hashcons_get_ctr : hashcons_st key CoqBigInt.t :=
-  st_get1.
+  t <- get;;
+  ret (find_opt_hashset hash eqb (snd t) k).
+Definition hashcons_get_ctr: hashcons_st key CoqBigInt.t :=
+  t <- get ;;
+  ret (fst t).
 Definition hashcons_add (k: key) : hashcons_st key unit :=
-  hashcons_bnd (fun h => st_set2 (add_hashset hash h k)) st_get2.
+  t <- get;;
+  put (fst t, add_hashset hash (snd t) k).
 Definition hashcons_incr : hashcons_st key unit :=
-  hashcons_bnd (fun i => st_set1 (CoqBigInt.succ i)) st_get1.
+  t <- get;;
+  put (CoqBigInt.succ (fst t), snd t).
 Definition hashcons_list {K A : Type} (l: list (@hashcons_st K A)) :
-  @hashcons_st K (list A) := st_listM l.
+  @hashcons_st K (list A) := listM hashcons_ret hashcons_bnd l.
 End HashCons.
 (*TODO: for now, notations*)
 
@@ -185,7 +201,30 @@ Definition hashcons_unit key := hashcons_st key unit.
 
 
 (*Monad transformers (kind of)*)
-Require Import ErrorMonad.
+
+(*Later, switch to Either monad from ExtLib*)
+Definition errorHashT (K A: Type) := (eitherT errtype 
+  (state (CoqBigInt.t * (hashset K))) A).
+Global Instance Monad_errorHashT K: Monad (errorHashT K) := Monad_eitherT _ (Monad_state _). 
+Global Instance MonadT_errorHashT K: MonadT (errorHashT K) (hashcons_st K) := 
+  MonadT_eitherT _ (Monad_state _). 
+Global Instance MonadState_errorHashT K: MonadState (CoqBigInt.t * (hashset K))
+  (errorHashT K) := MonadState_eitherT _ (Monad_state _) (MonadState_state _).
+Global Instance Exception_errorHashT K : MonadExc errtype (errorHashT K) :=
+  Exception_eitherT _ (Monad_state _).
+
+(*Global Instance MonadState_hashcons_st key : 
+  MonadState (CoqBigInt.t * hashset key) (hashcons_st key) := MonadState_state _.*)
+Definition errorHash_bnd {K a b} (f: a -> errorHashT K b) (m: errorHashT K a):
+  errorHashT K b := bind m f.
+Definition errorHash_ret {K a} (x: a) : errorHashT K a := ret x.
+Definition errorHash_lift {K a} (x: hashcons_st K a) : errorHashT K a := lift x.
+(*TODO: do we need this?*)
+Definition errorHash_lift2 {K a} (x: errorM a) : errorHashT K a := 
+  match x with
+  | inl e => raise e
+  | inr t => ret t
+  end.
 
 (*Ok, we do want a monad instance for (errorM (hashcons_st A))
   so we can use listM
@@ -194,11 +233,11 @@ Require Import ErrorMonad.
 (*For now, do 1 by 1*)
 (*Choose this order: state still exists, may have result*)
 (*Basically ExceptT on state monad*)
-Notation errorHashT K A := (exceptT (CoqBigInt.t * (@hashset K)) A).
+(*Notation errorHashT K A := (exceptT (CoqBigInt.t * (@hashset K)) A).
 (*Names for compatibility*)
 Notation errorHash_bnd := exceptT_bnd.
 Notation errorHash_ret := exceptT_ret.
-Notation errorHash_lift := exceptT_lift.
+Notation errorHash_lift := exceptT_lift.*)
 Definition errorHash_list {K A: Type} (l: list (@errorHashT K A)) :
  @errorHashT K (list A) :=
   listM errorHash_ret errorHash_bnd l.
